floyd/assert_lemmas.v
@@ -1160,7 +1160,7 @@ Abort. (* broken in CompCert 2.7 *)
 
 Lemma typed_false_cmp:
   forall op i j , 
-   typed_false tint (force_val (sem_cmp op tint tint true2 (Vint i) (Vint j))) ->
+   typed_false tint (force_val (sem_cmp op tint tint (Vint i) (Vint j))) ->
    Int.cmp (negate_comparison op) i j = true.
 Proof.
 intros.
@@ -1172,7 +1172,7 @@ Qed.
 
 Lemma typed_true_cmp:
   forall op i j, 
-   typed_true tint (force_val (sem_cmp op tint tint true2 (Vint i) (Vint j))) ->
+   typed_true tint (force_val (sem_cmp op tint tint (Vint i) (Vint j))) ->
    Int.cmp op i j = true.
 Proof.
 intros.
@@ -1228,7 +1228,7 @@ Qed.
 Lemma typed_false_cmp_repr:
   forall op i j, 
    repable_signed i -> repable_signed j -> 
-   typed_false tint (force_val (sem_cmp op tint tint true2
+   typed_false tint (force_val (sem_cmp op tint tint
                               (Vint (Int.repr i)) 
                               (Vint (Int.repr j)) )) ->
    Zcmp (negate_comparison op) i j.
@@ -1241,7 +1241,7 @@ Qed.
 Lemma typed_true_cmp_repr:
   forall op i j, 
    repable_signed i -> repable_signed j -> 
-   typed_true tint (force_val (sem_cmp op tint tint true2
+   typed_true tint (force_val (sem_cmp op tint tint
                               (Vint (Int.repr i)) 
                               (Vint (Int.repr j)) )) ->
    Zcmp op i j.
