floyd/entailer.v
@@ -656,45 +656,6 @@ apply prop_ext; intuition.
 Qed.
 Hint Rewrite offset_val_sizeof_hack3 : norm.
 
-(*
-Lemma cmpu_bool_ptr1: 
-  forall validptr c p, isptr p -> 
-     Val.cmpu_bool validptr c p (Vint Int.zero) 
-      = Val.cmp_different_blocks c.
-Proof.
-intros.  destruct p; try contradiction.  reflexivity.
-Qed.
-
-Lemma cmpu_bool_ptr2: 
-  forall validptr c p, isptr p -> 
-     Val.cmpu_bool validptr c (Vint Int.zero) p = Val.cmp_different_blocks c.
-Proof.
-intros. destruct p; try contradiction. reflexivity.
-Qed.
-Hint Rewrite cmpu_bool_ptr1 cmpu_bool_ptr2 using solve [auto] : norm.
-
-Lemma sem_cmp_pp_ptr1:
-  forall c p,  isptr p -> 
-   sem_cmp_pp c true2 p (Vint Int.zero) = 
-       option_map Val.of_bool (Val.cmp_different_blocks c).
-Proof.
-intros.
-unfold sem_cmp_pp; simpl. normalize.
-Qed.
-
-Lemma sem_cmp_pp_ptr2:
-  forall c p,  isptr p -> 
-   sem_cmp_pp c true2 (Vint Int.zero)  p= 
-       option_map Val.of_bool (Val.cmp_different_blocks c).
-Proof.
-intros.
-unfold sem_cmp_pp.
-normalize.
-Qed.
-
-Hint Rewrite sem_cmp_pp_ptr1 sem_cmp_pp_ptr2 using solve [auto] : norm.
-*)
-
 Ltac make_Vptr c :=
   let H := fresh in assert (isptr c) by auto;
   destruct c; try (contradiction H); clear H.
